Extend definability with matching mains
Matching the main programs will not only be the responsibility of the
compiler, but also, notably, of our definability scheme. It is somewhat
unsatisfying that Source and Intermediate levels have concepts of
program that are distinct enough that the definition needs to be
repeated at various levels.

RSC_DC_MD.v
@@ -325,7 +325,9 @@ Module Intermediate_Instance <: Intermediate_Sig.
 End Intermediate_Instance.
 
 Module Type Linker_Sig (Source : Source_Sig) (Intermediate : Intermediate_Sig).
-  Axiom  definability_with_linking :
+  Parameter matching_mains : Source.program -> Intermediate.program -> Prop.
+
+  Axiom definability_with_linking :
     forall p c b m,
       Intermediate.well_formed_program p ->
       Intermediate.well_formed_program c ->
@@ -337,6 +339,8 @@ Module Type Linker_Sig (Source : Source_Sig) (Intermediate : Intermediate_Sig).
     exists p' c',
       Source.prog_interface p' = Intermediate.prog_interface p /\
       Source.prog_interface c' = Intermediate.prog_interface c /\
+      matching_mains p' p /\
+      matching_mains c' c /\
       Source.well_formed_program p' /\
       Source.well_formed_program c' /\
       Source.closed_program (Source.program_link p' c') /\
@@ -345,6 +349,9 @@ Module Type Linker_Sig (Source : Source_Sig) (Intermediate : Intermediate_Sig).
 End Linker_Sig.
 
 Module Linker_Instance <: Linker_Sig (Source_Instance) (Intermediate_Instance).
+  Definition matching_mains :=
+    @RobustImp.Source.Definability.matching_mains.
+
   Definition definability_with_linking :=
     @RobustImp.Source.Definability.definability_with_linking.
 End Linker_Instance.
@@ -521,7 +528,8 @@ Section RSC_DC_MD_Section.
                 linkability_pcomp_Ct closedness Hbeh Hprefix0 Hnot_wrong')
       as [P' [Cs
          [Hsame_iface1 [Hsame_iface2
-         [well_formed_P' [well_formed_Cs [HP'Cs_closed [HP'_Cs_beh Hprefix1]]]]]]]].
+         [Hmains1 [Hmains2
+         [well_formed_P' [well_formed_Cs [HP'Cs_closed [HP'_Cs_beh Hprefix1]]]]]]]]]].
 
     move: HP'_Cs_beh Hprefix1.
     set beh := Terminates _.
